Get rid of the `invG` dependency on `lty2`.

theories/logic/model.v
@@ -11,29 +11,29 @@ From reloc Require Import prelude.tactics logic.spec_rules prelude.ctx_subst.
 From reloc Require Export logic.spec_ra.
 
 (** Semantic intepretation of types *)
-Record lty2 `{invG Σ} := Lty2 {
+Record lty2 Σ := Lty2 {
   lty2_car :> val → val → iProp Σ;
   lty2_persistent v1 v2 : Persistent (lty2_car v1 v2)
 }.
-Arguments Lty2 {_ _} _%I {_}.
-Arguments lty2_car {_ _} _ _ _ : simpl never.
+Arguments Lty2 {_} _%I {_}.
+Arguments lty2_car {_} _ _ _ : simpl never.
 Bind Scope lty_scope with lty2.
 Delimit Scope lty_scope with lty2.
 Existing Instance lty2_persistent.
 
 (* The COFE structure on semantic types *)
 Section lty2_ofe.
-  Context `{invG Σ}.
+  Context `{Σ : gFunctors}.
 
-  Instance lty2_equiv : Equiv lty2 := λ A B, ∀ w1 w2, A w1 w2 ≡ B w1 w2.
-  Instance lty2_dist : Dist lty2 := λ n A B, ∀ w1 w2, A w1 w2 ≡{n}≡ B w1 w2.
-  Lemma lty2_ofe_mixin : OfeMixin lty2.
-  Proof. by apply (iso_ofe_mixin (lty2_car : lty2 → (val -c> val -c> iProp Σ))). Qed.
-  Canonical Structure lty2C := OfeT lty2 lty2_ofe_mixin.
+  Instance lty2_equiv : Equiv (lty2 Σ) := λ A B, ∀ w1 w2, A w1 w2 ≡ B w1 w2.
+  Instance lty2_dist : Dist (lty2 Σ) := λ n A B, ∀ w1 w2, A w1 w2 ≡{n}≡ B w1 w2.
+  Lemma lty2_ofe_mixin : OfeMixin (lty2 Σ).
+  Proof. by apply (iso_ofe_mixin (lty2_car : lty2 Σ → (val -c> val -c> iProp Σ))). Qed.
+  Canonical Structure lty2C := OfeT (lty2 Σ) lty2_ofe_mixin.
 
   Global Instance lty2_cofe : Cofe lty2C.
   Proof.
-    apply (iso_cofe_subtype' (λ A : val -c> val -c> iProp Σ, ∀ w1 w2, Persistent (A w1 w2)) (@Lty2 _ _) lty2_car)=>//.
+    apply (iso_cofe_subtype' (λ A : val -c> val -c> iProp Σ, ∀ w1 w2, Persistent (A w1 w2)) (@Lty2 _) lty2_car)=>//.
     - apply _.
     - apply limit_preserving_forall=> w1.
       apply limit_preserving_forall=> w2.
@@ -41,7 +41,7 @@ Section lty2_ofe.
       intros n P Q HPQ. apply (HPQ w1 w2).
   Qed.
 
-  Global Instance lty2_inhabited : Inhabited lty2 := populate (Lty2 inhabitant).
+  Global Instance lty2_inhabited : Inhabited (lty2 Σ) := populate (Lty2 inhabitant).
 
   Global Instance lty2_car_ne n : Proper (dist n ==> (=) ==> (=) ==> dist n) lty2_car.
   Proof. by intros A A' ? w1 w2 <- ? ? <-. Qed.
@@ -49,13 +49,16 @@ Section lty2_ofe.
   Proof. solve_proper_from_ne. Qed.
 End lty2_ofe.
 
+Arguments lty2C : clear implicits.
+
 Section semtypes.
   Context `{relocG Σ}.
 
-  Implicit Types A B : lty2.
+  Implicit Types e : expr.
+  Implicit Types E : coPset.
+  Implicit Types A B : lty2 Σ.
 
-  Definition interp_expr (E : coPset) (e e' : expr)
-             (A : lty2) : iProp Σ :=
+  Definition interp_expr E e e' A : iProp Σ :=
     (∀ j K, j ⤇ fill K e'
     ={E,⊤}=∗ WP e {{ v, ∃ v', j ⤇ fill K (of_val v') ∗ A v v' }})%I.
 
@@ -67,26 +70,26 @@ Section semtypes.
     Proper ((≡) ==> (≡)) (interp_expr E e e').
   Proof. apply ne_proper=>n. apply _. Qed.
 
-  Definition lty2_unit : lty2 := Lty2 (λ w1 w2, ⌜ w1 = #() ∧ w2 = #() ⌝%I).
-  Definition lty2_bool : lty2 := Lty2 (λ w1 w2, ∃ b : bool, ⌜ w1 = #b ∧ w2 = #b ⌝)%I.
-  Definition lty2_int : lty2 := Lty2 (λ w1 w2, ∃ n : Z, ⌜ w1 = #n ∧ w2 = #n ⌝)%I.
+  Definition lty2_unit : lty2 Σ := Lty2 (λ w1 w2, ⌜ w1 = #() ∧ w2 = #() ⌝%I).
+  Definition lty2_bool : lty2 Σ := Lty2 (λ w1 w2, ∃ b : bool, ⌜ w1 = #b ∧ w2 = #b ⌝)%I.
+  Definition lty2_int : lty2 Σ := Lty2 (λ w1 w2, ∃ n : Z, ⌜ w1 = #n ∧ w2 = #n ⌝)%I.
 
-  Definition lty2_arr (A1 A2 : lty2) : lty2 := Lty2 (λ w1 w2,
+  Definition lty2_arr (A1 A2 : lty2 Σ) : lty2 Σ := Lty2 (λ w1 w2,
     □ ∀ v1 v2, A1 v1 v2 -∗ interp_expr ⊤ (App w1 v1) (App w2 v2) A2)%I.
 
-  Definition lty2_ref (A : lty2) : lty2 := Lty2 (λ w1 w2,
+  Definition lty2_ref (A : lty2 Σ) : lty2 Σ := Lty2 (λ w1 w2,
     ∃ l1 l2: loc, ⌜w1 = #l1⌝ ∧ ⌜w2 = #l2⌝ ∧
       inv (relocN .@ "ref" .@ (l1,l2)) (∃ v1 v2, l1 ↦ v1 ∗ l2 ↦ₛ v2 ∗ A v1 v2))%I.
 
-  Definition lty2_prod (A B : lty2) : lty2 := Lty2 (λ w1 w2,
+  Definition lty2_prod (A B : lty2 Σ) : lty2 Σ := Lty2 (λ w1 w2,
     ∃ v1 v2 v1' v2', ⌜w1 = (v1,v1')%V⌝ ∧ ⌜w2 = (v2,v2')%V⌝ ∧
         A v1 v2 ∗ B v1' v2')%I.
 
-  Definition lty2_sum (A B : lty2) : lty2 := Lty2 (λ w1 w2,
+  Definition lty2_sum (A B : lty2 Σ) : lty2 Σ := Lty2 (λ w1 w2,
     ∃ v1 v2, (⌜w1 = InjLV v1⌝ ∧ ⌜w2 = InjLV v2⌝ ∧ A v1 v2)
           ∨  (⌜w1 = InjRV v1⌝ ∧ ⌜w2 = InjRV v2⌝ ∧ B v1 v2))%I.
 
-  Definition lty2_rec1 (C : lty2C -n> lty2C) (rec : lty2) : lty2 :=
+  Definition lty2_rec1 (C : lty2C Σ -n> lty2C Σ) (rec : lty2 Σ) : lty2 Σ :=
     Lty2 (λ w1 w2, ▷ C rec w1 w2)%I.
   Instance lty2_rec1_contractive C : Contractive (lty2_rec1 C).
   Proof.
@@ -97,10 +100,10 @@ Section semtypes.
     simpl in HPQ; simpl. f_equiv. by apply C.
   Qed.
 
-  Definition lty2_rec (C : lty2C -n> lty2C) : lty2 := fixpoint (lty2_rec1 C).
+  Definition lty2_rec (C : lty2C Σ -n> lty2C Σ) : lty2 Σ := fixpoint (lty2_rec1 C).
 
-  Definition lty2_exists (C : lty2 → lty2) : lty2 := Lty2 (λ w1 w2,
-    ∃ A : lty2, C A w1 w2)%I.
+  Definition lty2_exists (C : lty2 Σ → lty2 Σ) : lty2 Σ := Lty2 (λ w1 w2,
+    ∃ A, C A w1 w2)%I.
 
   (** The lty2 constructors are non-expansive *)
   Instance lty2_prod_ne n : Proper (dist n ==> (dist n ==> dist n)) lty2_prod.
@@ -113,7 +116,7 @@ Section semtypes.
   Proof. solve_proper. Qed.
 
   Instance lty2_rec_ne n : Proper (dist n ==> dist n)
-                                   (lty2_rec : (lty2C -n> lty2C) -> lty2C).
+                                   (lty2_rec : (lty2C Σ -n> lty2C Σ) -> lty2C Σ).
   Proof.
     intros F F' HF.
     unfold lty2_rec, lty2_car.
@@ -123,7 +126,7 @@ Section semtypes.
     apply lty2_car_ne; eauto.
   Qed.
 
-  Lemma lty_rec_unfold (C : lty2C -n> lty2C) : lty2_rec C ≡ lty2_rec1 C (lty2_rec C).
+  Lemma lty_rec_unfold (C : lty2C Σ -n> lty2C Σ) : lty2_rec C ≡ lty2_rec1 C (lty2_rec C).
   Proof. apply fixpoint_unfold. Qed.
 
 End semtypes.
@@ -134,7 +137,7 @@ Infix "→" := lty2_arr : lty_scope.
 Notation "'ref' A" := (lty2_ref A) : lty_scope.
 
 (* The semantic typing judgment *)
-Definition env_ltyped2 `{relocG Σ} (Γ : gmap string lty2)
+Definition env_ltyped2 `{relocG Σ} (Γ : gmap string (lty2 Σ))
     (vs : gmap string (val*val)) : iProp Σ :=
   (⌜ ∀ x, is_Some (Γ !! x) ↔ is_Some (vs !! x) ⌝ ∧
   [∗ map] i ↦ Avv ∈ map_zip Γ vs, lty2_car Avv.1 Avv.2.1 Avv.2.2)%I.
@@ -221,8 +224,8 @@ Section refinement.
   Context `{relocG Σ}.
 
   Definition refines_def  (E : coPset)
-           (Γ : gmap string lty2)
-           (e e' : expr) (A : lty2) : iProp Σ :=
+           (Γ : gmap string (lty2 Σ))
+           (e e' : expr) (A : lty2 Σ) : iProp Σ :=
     (∀ vvs ρ, spec_ctx ρ -∗
               env_ltyped2 Γ vvs -∗
               interp_expr E (subst_map (fst <$> vvs) e)
@@ -253,7 +256,7 @@ Section semtypes_properties.
 
   (* The reference type relation is functional and injective.
      Thanks to Amin. *)
-  Lemma interp_ref_funct E (A : lty2) (l l1 l2 : loc) :
+  Lemma interp_ref_funct E (A : lty2 Σ) (l l1 l2 : loc) :
     ↑relocN ⊆ E →
     (ref A)%lty2 #l #l1 ∗ (ref A)%lty2 #l #l2
     ={E}=∗ ⌜l1 = l2⌝.
@@ -269,7 +272,7 @@ Section semtypes_properties.
     compute in Hfoo. eauto.
   Qed.
 
-  Lemma interp_ref_inj E (A : lty2) (l l1 l2 : loc) :
+  Lemma interp_ref_inj E (A : lty2 Σ) (l l1 l2 : loc) :
     ↑relocN ⊆ E →
     (ref A)%lty2 #l1 #l ∗ (ref A)%lty2 #l2 #l
     ={E}=∗ ⌜l1 = l2⌝.
@@ -285,7 +288,7 @@ Section semtypes_properties.
     compute in Hfoo. eauto.
   Qed.
 
-  Lemma interp_ret (A : lty2) E e1 e2 v1 v2 :
+  Lemma interp_ret (A : lty2 Σ) E e1 e2 v1 v2 :
     IntoVal e1 v1 →
     IntoVal e2 v2 →
     (|={E,⊤}=> A v1 v2)%I -∗ interp_expr E e1 e2 A.
@@ -298,8 +301,8 @@ End semtypes_properties.
 
 Section environment_properties.
   Context `{relocG Σ}.
-  Implicit Types A B : lty2.
-  Implicit Types Γ : gmap string lty2.
+  Implicit Types A B : lty2 Σ.
+  Implicit Types Γ : gmap string (lty2 Σ).
 
   Lemma env_ltyped2_lookup Γ vs x A :
     Γ !! x = Some A →
@@ -433,7 +436,7 @@ Section monadic.
     by rewrite !subst_map_fill /=.
   Qed.
 
-  Lemma refines_ret E Γ e1 e2 v1 v2 (A : lty2) :
+  Lemma refines_ret E Γ e1 e2 v1 v2 (A : lty2 Σ) :
     IntoVal e1 v1 →
     IntoVal e2 v2 →
     (|={E,⊤}=> A v1 v2) -∗ {E;Γ} ⊨ e1 << e2 : A.
